ReactorModel/Execution/Theorems/Variability/Basic.lean
@@ -1,0 +1,53 @@
+import ReactorModel.Execution.Theorems.Step.Basic
+import ReactorModel.Execution.Theorems.State
+import ReactorModel.Execution.Theorems.Variability.LoopModel
+
+open Classical Reactor
+
+namespace Execution
+
+-- Property (2) on page 10 of https://www.informatik.uni-bremen.de/agbs/jp/papers/trs_script.pdf.
+-- "The computation can perform only finitely many state changes in any finite time interval."
+--
+-- We formalize this as:
+-- For any initial execution state `s₁` and tag `g`, there exists a bound `b` on the length of
+-- executions which start at `s₁` and stay below `g`.
+--
+-- It is important that the bound `b` can depend on `s₁`, because otherwise it may be exeeded simply
+-- by the sheer number of reactions contained in the reactor of `s₁`, or by the number of events
+-- already present in its event queue.
+--
+-- Note: This property is parameterized over the reactor type (`α`), because finite variability is a
+--       property of the *model* of Reactors, and the given reactor type (or rather its accompanying
+--       type class instances) defines the model.
+def FiniteVariability (α) [Hierarchical α] : Prop :=
+  ∀ g s, ∃ b, ∀ {s' : State α} (e : Execution s s'),
+    (s'.tag < g) → e.length < b
+
+-- Properness of a finite reactor model is not sufficient for finite variability. This is a
+-- consequence of logical tags being super-dense.
+--
+-- Proof Idea: Construct a reactor with a reaction which always schedules and action for the
+--             current logical time. This only ever increases the micro-step, but not the time.
+theorem not_finitely_variable : ¬∀ (α) [Proper α] [Reactor.Finite α], FiniteVariability α := by
+  intro h
+  let s₁ : State LoopModel.Rtr := {
+    rtr := { act := true },
+    tag := ⟨0, 0⟩,
+    progress := ∅,
+    events
+      | .r => none
+      | .a => some <| .singleton ⟨0, 0⟩ true
+  }
+  have ⟨b, h⟩ := h _ ⟨1, 0⟩ s₁
+  let s₂ : State LoopModel.Rtr := {
+    rtr := { act := true },
+    tag := ⟨0, b⟩,
+    progress := ∅,
+    events
+      | .r => none
+      | .a => sorry -- TODO: The execution semantics don't include deleting old events.
+  }
+  let e : Execution s₁ s₂ := sorry -- TODO: Construct this recursively.
+  have hl : e.length = b := sorry
+  exact lt_irrefl b (hl ▸ h e Time.Tag.lt_of_lt_time)
