ReactorModel/Execution/Theorems/Variability/LoopModel.lean
@@ -1,0 +1,144 @@
+import ReactorModel.Objects.Reactor.Proper
+import ReactorModel.Objects.Reactor.Finite
+
+open Reactor
+
+namespace LoopModel
+
+inductive Ident where
+  | r
+  | a
+
+@[ext]
+structure Rtr where
+  act : Bool
+
+instance : Identifiable Rtr where
+  Id := Ident
+
+instance : Valued Rtr where
+  Val          := Bool
+  value.absent := false
+
+instance : Prioritizable Rtr where
+  Priority := Unit
+  order    := inferInstance
+
+def Rtr.rcn : Reaction Rtr where
+  deps _               := {⟨.act, .a⟩}
+  triggers             := {⟨.act, .a⟩}
+  prio                 := .unit
+  body inp             := [.act .a inp.tag.time true]
+  triggers_sub_in_deps := by simp_all
+  target_mem_deps      := by simp_all [Change.Normal.target]
+
+instance : Reactor Rtr where
+  get? rtr
+    | .rcn, .r => Rtr.rcn
+    | .act, .a => rtr.act
+    | _,    _  => none
+
+instance : Extensional Rtr where
+  ext_iff := by
+    intro rtr₁ rtr₂
+    constructor <;> intro h
+    case mp  => rw [h]
+    case mpr => ext; injection (by rw [h] : rtr₁{.act}{Ident.a} = rtr₂{.act}{Ident.a})
+
+instance : Hierarchical Rtr where
+  unique_ids := by
+    intro rtr cpt i
+    constructor
+    intro m₁ m₂
+    cases m₁
+    case root => cases m₂; rfl
+    case strict s =>
+      cases cpt
+      case rtr => cases s <;> contradiction
+      all_goals
+        cases m₂; cases s <;> cases ‹StrictMember ..› <;> try contradiction
+        next h₁ _ h₂ => have h := h₁ ▸ h₂; injection h with h; subst h; rfl
+
+instance : WellFounded Rtr where
+  wf := by
+    constructor; intro rtr₁
+    constructor; intro rtr₂ h
+    have ⟨_, _⟩ := h
+    contradiction
+
+instance : Updatable Rtr where
+  update rtr
+    | .act, .a, v => { act := v }
+    | _,    _,  _ => rtr
+
+instance : LawfulUpdatable Rtr where
+  lawful rtr cpt i v := by
+    cases cpt <;> cases i
+    case act.a =>
+      apply LawfulUpdate.update <| LawfulMemUpdate.final ?_ rfl rfl
+      intro cpt i h
+      cases cpt <;> cases i <;> try rfl
+      all_goals cases ‹Component.Valued› <;> try rfl
+      cases h <;> contradiction
+    all_goals
+      apply LawfulUpdate.notMem ?_ rfl
+      · constructor; intro m; cases m; cases ‹StrictMember _ _ _› <;> contradiction
+
+instance : Proper Rtr where
+  unique_ids     := Hierarchical.unique_ids
+  wf             := WellFounded.wf
+  update         := Updatable.update
+  lawful         := LawfulUpdatable.lawful
+  wellformed rtr := {
+    unique_inputs h₁ h₂ hi :=
+      -- Contradiction, we have two distinct ids which both map to `some` reaction.
+      sorry
+    ordered_prio _ h₁ h₂ hi :=
+      -- Contradiction, we have two distinct ids which both map to `some` reaction.
+      sorry
+    valid_deps hn hr hd := sorry
+  }
+
+instance : Finite Ident :=
+  .intro (n := 2) {
+    toFun
+      | .r => 0
+      | .a => 1
+    invFun
+      | 0 => .r
+      | 1 => .a
+    left_inv
+      | .r | .a => rfl
+    right_inv
+      | 0 | 1      => rfl
+      | ⟨_ + 2, _⟩ => by contradiction
+  }
+
+example {p : A → Prop} (h : ∀ x, ¬p x) : {a | p a} = ∅ := by
+  exact Set.subset_eq_empty h rfl
+
+instance : Reactor.Finite Rtr where
+  fin rtr cpt := by
+    cases cpt <;> try cases ‹Component.Valued›
+    case act =>
+      simp only [Partial.Finite, Partial.ids]
+      sorry -- This should hold because `Ident` is finite, so any set over `Ident` is finite.
+    case rcn =>
+      simp only [Partial.Finite, Partial.ids]
+      sorry -- This should hold because `Ident` is finite, so any set over `Ident` is finite.
+    case rtr =>
+      simp only [Partial.Finite, Partial.ids]
+      sorry -- The top level reactor is also counted.
+    case' inp => have h : rtr[.inp].ids = ∅ := ?_
+    case' out => have h : rtr[.out].ids = ∅ := ?_
+    case' stv => have h : rtr[.stv].ids = ∅ := ?_
+    all_goals
+      first
+        | simp only [Partial.Finite, h, Set.finite_empty]
+        | apply Set.subset_eq_empty ?_ rfl
+          intro i h
+          simp [Partial.ids, Hierarchical.obj?] at h
+          have ⟨_, ⟨_, _⟩, _⟩ := h
+          cases ‹Object _ _ _ _›; cases ‹Member _ _ _›; cases ‹StrictMember _ _ _› <;> contradiction
+
+end LoopModel
