ReactorModel/Execution/Theorems/Variability/Weak.lean
@@ -1,0 +1,21 @@
+import ReactorModel.Execution.Theorems.Step.Basic
+import ReactorModel.Execution.Theorems.State
+
+open Classical Reactor
+
+namespace Execution
+
+-- "Weak finite variability" restricts the notion of finite variability to a single logical time.
+-- That is, this property holds if for any given logical time `t`, there exists a bound on the
+-- length of execution traces which occur at tags `g` with time `g.time = t`. Stated differently,
+-- this means that you can't have infinitely many state changes between two microsteps of the same
+-- logical time.
+--
+-- TODO: This gives me ε/δ vibes. Does this alternation of ∃ and ∀ correspond to some existing
+--       notion like limits or convergence?
+def WeakFiniteVariability (α) [Hierarchical α] : Prop :=
+  ∀ t m s, ∃ b, ∀ {s' : State α} (e : Execution s s'),
+    (s.tag.time = t) → (s'.tag < ⟨t, m⟩) → e.length < b
+
+theorem weakly_finitely_variable [Proper α] [Reactor.Finite α] : WeakFiniteVariability α := by
+  sorry
